vale/code/arch/x64/interop/Vale.Wrapper.X64.GCM_IV.fsti
@@ -48,5 +48,5 @@ val compute_iv
   (ensures fun h0 _ h1 ->
     B.modifies (B.loc_buffer j0_b `B.loc_union` B.loc_buffer extra_b) h0 h1 /\
     le_bytes_to_quad32 (seq_uint8_to_seq_nat8 (B.as_seq h1 j0_b)) ==
-      compute_iv_BE (aes_encrypt_LE a (Ghost.reveal key) (Mkfour 0 0 0 0))
+      compute_iv_BE (reverse_bytes_quad32 (aes_encrypt_LE a (Ghost.reveal key) (Mkfour 0 0 0 0)))
                     (seq_uint8_to_seq_nat8 (B.as_seq h0 iv_b)))
